docs for Basic

src/Std/Data/Iterators/Basic.lean
@@ -13,15 +13,106 @@ namespace Std
 
 namespace Iterators
 
-structure IterM {α : Type w} (m : Type w → Type w') (β : Type v) : Type w where
+/--
+An iterator that sequentially emits values of type `β` in the monad `m`. It may be finite
+or infinite.
+
+See the root module `Std.Data.Iterators` for a more comprehensive overview over the iterator
+framework.
+
+See `Std.Data.Iterators.Producers` for ways to iterate over common data structures.
+By convention, the monadic iterator associated with an object can be obtained via dot notation.
+For example, `List.iterM IO` creates an iterator over a list in the monad `IO`.
+
+See `Std.Data.Iterators.Consumers` for ways to use an iterator. For example, `it.toList` will
+convert a provably finite iterator `it` into a list and `it.allowNontermination.toList` will
+do so even if finiteness cannot be proved. It is also always possible to manually iterate using
+`it.step`, relying on the termination measures `it.finitelyManySteps` and `it.finitelyManySkips`.
+
+See `Std.Data.Iterators.Combinators` for ways to compose iterators. For example, `it.map f` is
+the iterator that applies a function `f` to every value emitted by `it`.
+
+See `Iter` for a more convenient interface in case that no monadic effects are needed (`m = Id`).
+
+Internally, `IterM m β` wraps an element of type `α` containing state information.
+The type `α` determines the implementation of the iterator using a typeclass mechanism.
+The concrete typeclass implementing the iterator is `Iterator α m β`.
+
+When using combinators, `α` can become very complicated. It is an implicit parameter
+of `α` so that the pretty printer will not print this large type by default. If a declaration
+returns an iterator, the following will not work:
+
+```lean
+def x : IterM IO Nat := [1, 2, 3].iterM IO
+```
+
+Instead the declaration type needs to be completely omitted:
+
+```lean
+def x := [1, 2, 3].iterM IO
+
+-- if you want to ensure that `x` is an iterator in `IO` emitting `Nat`
+def x := ([1, 2, 3].iterM IO : IterM IO Nat)
+```
+-/
+structure IterM {α : Type w} (m : Type w → Type w') (β : Type w) : Type w where
   inner : α
 
-structure Iter {α : Type w} (β : Type v) : Type w where
+/--
+An iterator that sequentially emits values of type `β`. It may be finite
+or infinite.
+
+See the root module `Std.Data.Iterators` for a more comprehensive overview over the iterator
+framework.
+
+See `Std.Data.Iterators.Producers` for ways to iterate over common data structures.
+By convention, the monadic iterator associated with an object can be obtained via dot notation.
+For example, `List.iterM IO` creates an iterator over a list in the monad `IO`.
+
+See `Std.Data.Iterators.Consumers` for ways to use an iterator. For example, `it.toList` will
+convert a provably finite iterator `it` into a list and `it.allowNontermination.toList` will
+do so even if finiteness cannot be proved. It is also always possible to manually iterate using
+`it.step`, relying on the termination measures `it.finitelyManySteps` and `it.finitelyManySkips`.
+
+See `Std.Data.Iterators.Combinators` for ways to compose iterators. For example, `it.map f` is
+the iterator that applies a function `f` to every value emitted by `it`.
+
+See `IterM` for iterators that operate in a monad.
+
+Internally, `Iter β` wraps an element of type `α` containing state information.
+The type `α` determines the implementation of the iterator using a typeclass mechanism.
+The concrete typeclass implementing the iterator is `Iterator α m β`.
+
+When using combinators, `α` can become very complicated. It is an implicit parameter
+of `α` so that the pretty printer will not print this large type by default. If a declaration
+returns an iterator, the following will not work:
+
+```lean
+def x : Iter Nat := [1, 2, 3].iter
+```
+
+Instead the declaration type needs to be completely omitted:
+
+```lean
+def x := [1, 2, 3].iter
+
+-- if you want to ensure that `x` is an iterator emitting `Nat`
+def x := ([1, 2, 3].iter : Iter Nat)
+```
+-/
+structure Iter {α : Type w} (β : Type w) : Type w where
   inner : α
 
+/--
+Converts a pure iterator (`Iter β`) into a monadic iterator (`IterM Id β`) in the
+identity monad `Id`.
+-/
 def Iter.toIterM {α : Type w} {β : Type w} (it : Iter (α := α) β) : IterM (α := α) Id β :=
   ⟨it.inner⟩
 
+/--
+Converts a monadic iterator (`IterM Id β`) over `Id` into a pure iterator (`Iter β`).
+-/
 def IterM.toPureIter {α : Type w} {β : Type w} (it : IterM (α := α) Id β) : Iter (α := α) β :=
   ⟨it.inner⟩
 
@@ -39,18 +130,43 @@ section IterStep
 
 variable {α : Type u} {β : Type w}
 
+/--
+`IterStep α β` represents a step taken by an iterator (`Iter β` or `IterM m β`).
+-/
 inductive IterStep (α β) where
-| yield : (it : α) → (b : β) → IterStep α β
-| skip : (a : α) → IterStep α β
-| done : IterStep α β
+  /--
+  `IterStep.yield it out` describes the situation that an iterator emits `out` and provides `it`
+  as the succeeding iterator.
+  -/
+  | yield : (it : α) → (out : β) → IterStep α β
+  /--
+  `IterStep.skip it` describes the situation that an iterator does not emit anything in this
+  iteration and provides `it'` as the succeeding iterator.
 
+  Allowing `skip` steps is necessary to generate efficient code from a loop over an iterator.
+  -/
+  | skip : (it : α) → IterStep α β
+  /--
+  `IterStep.done` describes the situation that an iterator has finished and will neither emit
+  more values nor cause any monadic effects. In this case, no succeeding iterator is provided.
+  -/
+  | done : IterStep α β
+
+/--
+Returns the succeeding iterator stored in an iterator step or `none` if the step is `.done`
+and the iterator has finished.
+-/
 def IterStep.successor : IterStep α β → Option α
   | .yield it _ => some it
   | .skip it => some it
   | .done => none
 
+/--
+Applies functions to the succeeding iterator and the emitted value stored in an `IterStep`.
+-/
 @[always_inline, inline]
-def IterStep.map {α' : Type u'} {β' : Type v'} (f : α → α') (g : β → β') : IterStep α β → IterStep α' β'
+def IterStep.map {α' : Type u'} {β' : Type v'} (f : α → α') (g : β → β') :
+    IterStep α β → IterStep α' β'
   | .yield it out => .yield (f it) (g out)
   | .skip it => .skip (f it)
   | .done => .done
@@ -86,27 +202,43 @@ theorem IterStep.successor_map {α' : Type u'} {β' : Type v'} {f : α → α'} 
     (step.map f g).successor = step.successor.elim none (some <| f ·) := by
   cases step <;> rfl
 
+/--
+A variant of `IterStep` that bundles the step together with a proof that it is "plausible".
+The plausibility predicate will later be chosen to assert that a state is a plausible successor
+of another state. Having this proof bundled up with the step is important for termination proofs.
+
+See `IterM.Step` and `Iter.Step` for the concrete choice of the plausibility predicate.
+-/
 def PlausibleIterStep (plausible_step : IterStep α β → Prop) := Subtype plausible_step
 
+/--
+Match pattern for the `yield` case. See also `IterStep.yield`.
+-/
 @[match_pattern]
 def PlausibleIterStep.yield {plausible_step : IterStep α β → Prop}
     (it' : α) (out : β) (h : plausible_step (.yield it' out)) : PlausibleIterStep plausible_step :=
   ⟨.yield it' out, h⟩
 
+/--
+Match pattern for the `skip` case. See also `IterStep.skip`.
+-/
 @[match_pattern]
 def PlausibleIterStep.skip {plausible_step : IterStep α β → Prop}
     (it' : α) (h : plausible_step (.skip it')) : PlausibleIterStep plausible_step :=
   ⟨.skip it', h⟩
 
+/--
+Match pattern for the `done` case. See also `IterStep.done`.
+-/
 @[match_pattern]
 def PlausibleIterStep.done {plausible_step : IterStep α β → Prop}
     (h : plausible_step .done) : PlausibleIterStep plausible_step :=
   ⟨.done, h⟩
 
-def PlausibleIterStep.successor (plausible_step : IterStep α β → Prop)
-    (step : PlausibleIterStep plausible_step) : Option α :=
-  step.val.successor
-
+/--
+Applies functions to the succeeding iterator and the emitted value stored in a `PlausibleIterStep`.
+See also `IterStep.map`.
+-/
 @[always_inline, inline]
 def PlausibleIterStep.map {plausible_step : IterStep α β → Prop}
     {α' : Type u'} {β' : Type v'} (f : α → α') (g : β → β') (new_plausible_step : IterStep α' β' → Prop)
@@ -122,51 +254,82 @@ theorem PlausibleIterStep.map_id {plausible_step : IterStep α β → Prop}
 
 end IterStep
 
-section Typeclasses
+/--
+The typeclass providing the step function of an iterator in `Iter (α := α) β` or
+`IterM (α := α) m β`.
 
+In order to allow intrinsic termination proofs when iterating with the `step` function, the
+step object is bundled with a proof that it is a "plausible" step for the given current iterator.
+-/
 class Iterator (α : Type w) (m : Type w → Type w') (β : outParam (Type w)) where
   plausible_step : IterM (α := α) m β → IterStep (IterM (α := α) m β) β → Prop
   step : (it : IterM (α := α) m β) → m (PlausibleIterStep <| plausible_step it)
 
-end Typeclasses
-
 section Monadic
 
+/--
+Converts wraps the state of an iterator into an `IterM` object.
+-/
 @[always_inline, inline]
-def toIter {α : Type w} (it : α) (m : Type w → Type w') (β : Type w) :
+def toIterM {α : Type w} (it : α) (m : Type w → Type w') (β : Type w) :
     IterM (α := α) m β :=
   ⟨it⟩
 
 @[simp]
-theorem toIter_inner {α m β} (it : IterM (α := α) m β) :
-    toIter it.inner m β = it :=
+theorem toIterM_inner {α m β} (it : IterM (α := α) m β) :
+    toIterM it.inner m β = it :=
   rfl
 
 @[simp]
-theorem inner_toIter {α m β} (it : α) :
-    (toIter it m β).inner = it :=
+theorem inner_toIterM {α m β} (it : α) :
+    (toIterM it m β).inner = it :=
   rfl
 
+/--
+Asserts that certain step is plausibly the successor of a given iterator. What "plausible" means
+is up to the `Iterator` instance but it should be strong enough to allow termination proofs.
+-/
 abbrev IterM.plausible_step {α : Type w} {m : Type w → Type w'} {β : Type w} [Iterator α m β] :
     IterM (α := α) m β → IterStep (IterM (α := α) m β) β → Prop :=
   Iterator.plausible_step (α := α) (m := m)
 
+/--
+The type of the step object returned by `IterM.step`, containing an `IterStep`
+and a proof that this is a plausible step for the given iterator.
+-/
 abbrev IterM.Step {α : Type w} {m : Type w → Type w'} {β : Type w} [Iterator α m β]
     (it : IterM (α := α) m β) :=
   PlausibleIterStep it.plausible_step
 
+/--
+Asserts that a certain output value could plausibly be emitted by the given iterator in its next
+step.
+-/
 def IterM.plausible_output {α : Type w} {m : Type w → Type w'} {β : Type w} [Iterator α m β]
     (it : IterM (α := α) m β) (out : β) : Prop :=
   ∃ it', it.plausible_step (.yield it' out)
 
+/--
+Asserts that a certain iterator `it'` could plausibly be the directly succeeding iterator of another
+given iterator `it`.
+-/
 def IterM.plausible_successor_of {α : Type w} {m : Type w → Type w'} {β : Type w} [Iterator α m β]
     (it' it : IterM (α := α) m β) : Prop :=
   ∃ step, step.successor = some it' ∧ it.plausible_step step
 
-def IterM.plausible_skip_successor_of {α : Type w} {m : Type w → Type w'} {β : Type w} [Iterator α m β]
-    (it' it : IterM (α := α) m β) : Prop :=
+/--
+Asserts that a certain iterator `it'` could plausibly be the directly succeeding iterator of another
+given iterator `it` while no value is emitted (see `IterStep.skip`).
+-/
+def IterM.plausible_skip_successor_of {α : Type w} {m : Type w → Type w'} {β : Type w}
+    [Iterator α m β] (it' it : IterM (α := α) m β) : Prop :=
   it.plausible_step (.skip it')
 
+/--
+Makes a single step with the given iterator `it`, potentially emitting a value and providing a
+succeeding iterator. If this function is used recursively, termination can sometimes be proved with
+the termination measures `it.finitelyManySteps` and `it.finitelyManySkips`.
+-/
 def IterM.step {α : Type w} {m : Type w → Type w'} {β : Type w} [Iterator α m β]
     (it : IterM (α := α) m β) : m it.Step :=
   Iterator.step it
@@ -175,28 +338,52 @@ end Monadic
 
 section Pure
 
+/--
+Asserts that certain step is plausibly the successor of a given iterator. What "plausible" means
+is up to the `Iterator` instance but it should be strong enough to allow termination proofs.
+-/
 def Iter.plausible_step {α : Type w} {β : Type w} [Iterator α Id β]
     (it : Iter (α := α) β) (step : IterStep (Iter (α := α) β) β) : Prop :=
   it.toIterM.plausible_step (step.map Iter.toIterM id)
 
+/--
+The type of the step object returned by `Iter.step`, containing an `IterStep`
+and a proof that this is a plausible step for the given iterator.
+-/
 def Iter.Step {α : Type w} {β : Type w} [Iterator α Id β] (it : Iter (α := α) β) :=
   PlausibleIterStep (Iter.plausible_step it)
 
+/--
+Asserts that a certain output value could plausibly be emitted by the given iterator in its next
+step.
+-/
 def Iter.plausible_output {α : Type w} {β : Type w} [Iterator α Id β]
     (it : Iter (α := α) β) (out : β) : Prop :=
   ∃ it', it.plausible_step (.yield it' out)
 
+/--
+Asserts that a certain iterator `it'` could plausibly be the directly succeeding iterator of another
+given iterator `it`.
+-/
 def Iter.plausible_successor_of {α : Type w} {β : Type w} [Iterator α Id β]
     (it' it : Iter (α := α) β) : Prop :=
   ∃ step, step.successor = some it' ∧ it.plausible_step step
 
+/--
+Asserts that a certain iterator `it'` could plausibly be the directly succeeding iterator of another
+given iterator `it` while no value is emitted (see `IterStep.skip`).
+-/
 def Iter.plausible_skip_successor_of {α : Type w} {β : Type w} [Iterator α Id β]
     (it' it : Iter (α := α) β) : Prop :=
   it.plausible_step (.skip it')
 
+/--
+Makes a single step with the given iterator `it`, potentially emitting a value and providing a
+succeeding iterator. If this function is used recursively, termination can sometimes be proved with
+the termination measures `it.finitelyManySteps` and `it.finitelyManySkips`.
+-/
 @[always_inline, inline]
-def Iter.step {α : Type w} {β : Type w} [Iterator α Id β]
-    (it : Iter (α := α) β) : it.Step := by
+def Iter.step {α β : Type w} [Iterator α Id β] (it : Iter (α := α) β) : it.Step := by
   refine it.toIterM.step.run.map IterM.toPureIter id _ ?_
   intro step hp
   simp only [Iter.plausible_step, IterStep.map_map, id_eq, IterStep.map_id', toIterM_toPureIter, hp]
@@ -205,13 +392,27 @@ end Pure
 
 section Finite
 
-class Finite (α m) [Iterator α m β] : Prop where
+/--
+`Finite α m` asserts that `IterM (α := α) m` terminates after finitely many steps. Technically,
+this means that the relation of plausible successors is well-founded.
+Given this typeclass, termination proofs for well-founded recursion over an iterator `it` can use
+`it.finitelyManySteps` as a termination measure.
+-/
+class Finite (α : Type w) (m : Type w → Type w') {β : Type w} [Iterator α m β] : Prop where
   wf : WellFounded (IterM.plausible_successor_of (α := α) (m := m))
 
+/--
+This type is a wrapper around `IterM` so that it becomes a useful termination measure for
+recursion over finite iterators. See also `IterM.finitelyManySteps` and `Iter.finitelyManySteps`.
+-/
 structure IterM.TerminationMeasures.Finite
     (α : Type w) (m : Type w → Type w') {β : Type w} [Iterator α m β] where
   it : IterM (α := α) m β
 
+/--
+The relation of plausible successors on `IterM.TerminationMeasures.Finite`. It is well-founded
+if there is a `Finite` instance.
+-/
 def IterM.TerminationMeasures.Finite.rel
     {α : Type w} {m : Type w → Type w'} {β : Type w} [Iterator α m β] :
     TerminationMeasures.Finite α m → TerminationMeasures.Finite α m → Prop :=
@@ -222,16 +423,25 @@ instance {α : Type w} {m : Type w → Type w'} {β : Type w} [Iterator α m β]
   rel := IterM.TerminationMeasures.Finite.rel
   wf := (InvImage.wf _ Finite.wf).transGen
 
+/--
+Termination measure to be used in well-founded recursive functions recursing over a finite iterator
+(see also `Finite`).
+-/
 def IterM.finitelyManySteps {α : Type w} {m : Type w → Type w'} {β : Type w} [Iterator α m β]
     [Finite α m] (it : IterM (α := α) m β) : IterM.TerminationMeasures.Finite α m :=
   ⟨it⟩
 
+/--
+This theorem is used by a `decreasing_trivial` extension. It powers automatic termination proofs
+with `IterM.finitelyManySteps`.
+-/
 theorem IterM.TerminationMeasures.Finite.rel_of_yield
     {α : Type w} {m : Type w → Type w'} {β : Type w} [Iterator α m β]
     {it it' : IterM (α := α) m β} {out : β} (h : it.plausible_step (.yield it' out)) :
     rel ⟨it'⟩ ⟨it⟩ := by
   exact .single ⟨_, rfl, h⟩
 
+@[inherit_doc IterM.TerminationMeasures.Finite.rel_of_yield]
 theorem IterM.TerminationMeasures.Finite.rel_of_skip
     {α : Type w} {m : Type w → Type w'} {β : Type w} [Iterator α m β]
     {it it' : IterM (α := α) m β} (h : it.plausible_step (.skip it')) :
@@ -243,16 +453,22 @@ macro_rules | `(tactic| decreasing_trivial) => `(tactic|
   | exact IterM.TerminationMeasures.Finite.rel_of_yield ‹_›
   | exact IterM.TerminationMeasures.Finite.rel_of_skip ‹_›)
 
+@[inherit_doc IterM.finitelyManySteps]
 def Iter.finitelyManySteps {α : Type w} {β : Type w} [Iterator α Id β] [Finite α Id]
     (it : Iter (α := α) β) : IterM.TerminationMeasures.Finite α Id :=
   it.toIterM.finitelyManySteps
 
+/--
+This theorem is used by a `decreasing_trivial` extension. It powers automatic termination proofs
+with `IterM.finitelyManySteps`.
+-/
 theorem Iter.TerminationMeasures.Finite.rel_of_yield
     {α : Type w} {β : Type w} [Iterator α Id β]
     {it it' : Iter (α := α) β} {out : β} (h : it.plausible_step (.yield it' out)) :
     IterM.TerminationMeasures.Finite.rel ⟨it'.toIterM⟩ ⟨it.toIterM⟩ :=
   IterM.TerminationMeasures.Finite.rel_of_yield h
 
+@[inherit_doc Iter.TerminationMeasures.Finite.rel_of_yield]
 theorem Iter.TerminationMeasures.Finite.rel_of_skip
     {α : Type w} {β : Type w} [Iterator α Id β]
     {it it' : Iter (α := α) β} (h : it.plausible_step (.skip it')) :
@@ -268,13 +484,28 @@ end Finite
 
 section Productive
 
+/--
+`Productive α m` asserts that `IterM (α := α) m` terminates or emits a value after finitely many
+skips. Technically, this means that the relation of plausible successors during skips is
+well-founded.
+Given this typeclass, termination proofs for well-founded recursion over an iterator `it` can use
+`it.finitelyManySkips` as a termination measure.
+-/
 class Productive (α m) {β} [Iterator α m β] : Prop where
   wf : WellFounded (IterM.plausible_skip_successor_of (α := α) (m := m))
 
+/--
+This type is a wrapper around `IterM` so that it becomes a useful termination measure for
+recursion over productive iterators. See also `IterM.finitelyManySkips` and `Iter.finitelyManySkips`.
+-/
 structure IterM.TerminationMeasures.Productive
     (α : Type w) (m : Type w → Type w') {β : Type w} [Iterator α m β] where
   it : IterM (α := α) m β
 
+/--
+The relation of plausible successors while skipping on `IterM.TerminationMeasures.Productive`.
+It is well-founded if there is a `Productive` instance.
+-/
 def IterM.TerminationMeasures.Productive.rel
     {α : Type w} {m : Type w → Type w'} {β : Type w} [Iterator α m β] :
     TerminationMeasures.Productive α m → TerminationMeasures.Productive α m → Prop :=
@@ -285,10 +516,18 @@ instance {α : Type w} {m : Type w → Type w'} {β : Type w} [Iterator α m β]
   rel := IterM.TerminationMeasures.Productive.rel
   wf := (InvImage.wf _ Productive.wf).transGen
 
+/--
+Termination measure to be used in well-founded recursive functions recursing over a productive
+iterator (see also `Productive`).
+-/
 def IterM.finitelyManySkips {α : Type w} {m : Type w → Type w'} {β : Type w} [Iterator α m β]
     [Productive α m] (it : IterM (α := α) m β) : IterM.TerminationMeasures.Productive α m :=
   ⟨it⟩
 
+/--
+This theorem is used by a `decreasing_trivial` extension. It powers automatic termination proofs
+with `IterM.finitelyManySkips`.
+-/
 theorem IterM.TerminationMeasures.Productive.rel_of_skip
     {α : Type w} {m : Type w → Type w'} {β : Type w} [Iterator α m β]
     {it it' : IterM (α := α) m β} (h : it.plausible_step (.skip it')) :
@@ -298,10 +537,15 @@ theorem IterM.TerminationMeasures.Productive.rel_of_skip
 macro_rules | `(tactic| decreasing_trivial) => `(tactic|
   exact IterM.TerminationMeasures.Productive.rel_of_skip ‹_›)
 
+@[inherit_doc IterM.finitelyManySkips]
 def Iter.finitelyManySkips {α : Type w} {β : Type w} [Iterator α Id β] [Productive α Id]
     (it : Iter (α := α) β) : IterM.TerminationMeasures.Productive α Id :=
   it.toIterM.finitelyManySkips
 
+/--
+This theorem is used by a `decreasing_trivial` extension. It powers automatic termination proofs
+with `Iter.finitelyManySkips`.
+-/
 theorem Iter.TerminationMeasures.Productive.rel_of_skip
     {α : Type w} {β : Type w} [Iterator α Id β]
     {it it' : Iter (α := α) β} (h : it.plausible_step (.skip it')) :
